theories/ArityAnnotate/Base.v
@@ -4,7 +4,7 @@ From LambdaWeb Require Import ANF.
 (* We annotate function values with some Exposed web id based on their arities. *)
 Definition arity_to_web (n : nat) : web := Pos.of_nat n.
 
-(* We annotate constructor values with a single Exposed web id. *)
+(* We annotate constructor values with a single Exposed web id, since the sum and prod types get merged together in the language definition. But this matches with CertiCoq. *)
 (* Annotate constructor values with `wc`.
    This works since closure and constructor values live in different web universes. *)
 Definition wc := arity_to_web 0.
